RocqOfRust/revm/revm_interpreter/instructions/simulate/table.v
@@ -21,6 +21,7 @@ Require Import revm.revm_interpreter.instructions.links.block_info.
 Require Import revm.revm_interpreter.instructions.links.contract.call.
 Require Import revm.revm_interpreter.instructions.links.contract.call_code.
 Require Import revm.revm_interpreter.instructions.links.contract.delegate_call.
+Require Import revm.revm_interpreter.instructions.links.contract.static_call.
 Require Import revm.revm_interpreter.instructions.links.control.jump.
 Require Import revm.revm_interpreter.instructions.links.control.jumpdest.
 Require Import revm.revm_interpreter.instructions.links.control.jumpi.
@@ -161,6 +162,16 @@ Module FragmentInstructionTable.
       (run_host : Host.Run H H_types) :
       Function1.t (InstructionContext.t H WIRE WIRE_types) unit :=
     Function1.of_run (fun context => run_delegate_call run_types run_host context).
+
+  Definition static_call_function
+      {WIRE H : Set} `{Link WIRE} `{Link H}
+      {WIRE_types : InterpreterTypes.Types.t}
+      `{InterpreterTypes.Types.AreLinks WIRE_types}
+      {H_types : Host.Types.t} `{Host.Types.AreLinks H_types}
+      (run_types : InterpreterTypes.Run WIRE WIRE_types)
+      (run_host : Host.Run H H_types) :
+      Function1.t (InstructionContext.t H WIRE WIRE_types) unit :=
+    Function1.of_run (fun context => run_static_call run_types run_host context).
 
   Definition add_function
       {WIRE H : Set} `{Link WIRE} `{Link H}
@@ -1048,11 +1059,15 @@ Module FragmentInstructionTable.
         (ArrayPair.Build_t
           {| Instruction.fn_ := delegate_call_function run_InterpreterTypes_for_WIRE run_host;
              Instruction.static_gas := {| Integer.value := 0 |} |}
-          (prepend_repeat unknown_instruction 8 3
+          (prepend_repeat unknown_instruction 5 6
+            (ArrayPair.Build_t
+              {| Instruction.fn_ := static_call_function run_InterpreterTypes_for_WIRE run_host;
+                 Instruction.static_gas := {| Integer.value := 0 |} |}
+          (prepend_repeat unknown_instruction 2 3
             (ArrayPair.Build_t
               {| Instruction.fn_ := revert_function (H := H) run_InterpreterTypes_for_WIRE;
                  Instruction.static_gas := {| Integer.value := 0 |} |}
-              (ArrayPairs.repeat unknown_instruction 2))))))) in
+              (ArrayPairs.repeat unknown_instruction 2))))))))) in
     let tail_after_push0 :
         ArrayPairs.t (Instruction.t WIRE H WIRE_types) 161 :=
       ArrayPair.Build_t
