RocqOfRust/revm/revm_interpreter/interpreter/links/runtime_flags.v
@@ -1,0 +1,16 @@
+Require Import links.RocqOfRust.
+Require Import revm.revm_primitives.links.hardfork.
+
+Module RuntimeFlags.
+  RocqOfRustLinkRecord "revm_interpreter::interpreter::runtime_flags::RuntimeFlags" := {
+    is_static : bool;
+    spec_id : SpecId.t;
+  }.
+
+  Definition non_static (spec : SpecId.t) : t := {|
+    is_static := false;
+    spec_id := spec;
+  |}.
+
+End RuntimeFlags.
+Export (hints) RuntimeFlags.
